Kami/Ex/SCMMTrace.v
@@ -1,0 +1,52 @@
+Require Import Ascii Bool String List.
+Require Import Lib.CommonTactics Lib.Indexer Lib.ilist Lib.Word Lib.Struct Lib.FMap.
+Require Import Kami.Syntax Kami.Notations.
+Require Import Kami.Semantics Kami.Specialize Kami.Duplicate.
+Require Import Kami.Wf Kami.Tactics.
+Require Import Ex.MemTypes Ex.SC.
+
+Set Implicit Arguments.
+
+Open Scope fmap.
+
+Section MMIOLabel.
+  Variable addrSize: nat.
+  Variable dataBytes: nat.
+
+  Inductive MMIOLabelT :=
+  | MMIOSilent
+  | MMIOLd (addr: type (Bit addrSize)) (val: type (Data dataBytes))
+  | MMIOSt (addr: type (Bit addrSize)) (val: type (Data dataBytes)).
+
+  Definition MMIOLabelR (lbl: LabelT) (mlbl: MMIOLabelT): Prop.
+  Proof.
+    refine (match lbl.(defs)@["mmioExec"] with
+            | Some sv => _
+            | None => mlbl = MMIOSilent
+            end).
+    destruct sv as [[argT retT] [argV retV]].
+    destruct (decKind argT (Struct (RqFromProc addrSize dataBytes)));
+      [subst|exact False].
+    destruct (decKind retT (Struct (RsToProc dataBytes)));
+      [subst|exact False].
+
+    destruct (argV (Fin.FS Fin.F1)).
+    - (* MMIO-store *)
+      exact (mlbl = MMIOSt (argV Fin.F1) (argV (Fin.FS (Fin.FS Fin.F1)))).
+    - (* MMIO-load *)
+      exact (mlbl = MMIOLd (argV Fin.F1) (retV Fin.F1)).
+  Defined.
+
+  Definition MMIOTrace := list MMIOLabelT.
+
+  Inductive MMIOTraceR: LabelSeqT -> MMIOTrace -> Prop :=
+  | MMIOTraceRNil: MMIOTraceR nil nil
+  | MMIOTraceRCons:
+      forall tr mtr lbl mlbl,
+        MMIOTraceR tr mtr -> MMIOLabelR lbl mlbl ->
+        MMIOTraceR (lbl :: tr) (mlbl :: mtr).
+  
+End MMIOLabel.
+
+Close Scope fmap.
+
